A1/test.dfy
@@ -1,29 +1,29 @@
 // Find minimum element in the array between left and right
-function method findMin (a: array<int>, left: int, right: int): int
+function method findMax (a: array<int>, left: int, right: int): int
     reads a;
     decreases right - left;
     requires a != null && a.Length > 0;
     requires 0 <= left <= right < a.Length;
     ensures  0 <= left <= right < a.Length;
+    ensures 0 <= findMax(a, left, right) < a.Length;
 {
     if (left < right) then 
         if (a[left] < a[right]) then 
-            findMin(a, left, right - 1) 
-        else findMin(a, left + 1, right) 
-    else left
+            findMax(a, left + 1, right) 
+        else findMax(a, left, right - 1) 
+    else 0
 }
 
-method stoogeSort(a: array <int>, left: int, right: int) 
+method random(a: array <int>, left: int, right: int) 
     decreases right - left;
     requires a != null && a.Length > 0;
     requires 0 <= left <= right < a.Length;
-    requires 0 <= findMin(a, left, right) < a.Length;
+    requires 0 <= findMax(a, left, right) < a.Length;
     ensures 0 <= left <= right < a.Length;
 {
     if (left + 1 >= right) {
         return;
     }
-    stoogeSort(a, left, right - 1); 
-    stoogeSort(a, left + 1, right);
+    random(a, left, right - 1); 
+    random(a, left + 1, right);
 }
-
